add `analyze_program` to liveness analysis

extract/main.ml
@@ -5,16 +5,10 @@ let vm_new () = Vm (Nil, Nil);;
 let block_new ps is j = Lazy.from_val (
   Block (ps, is, Lazy.from_val j)
 );;
-
-let rec program_new bs =
-  match bs with
-  | [] -> Nil
-  | x :: xs -> Cons (x, (program_new xs))
-;;
+let program_new = block_new;;
 
 let vm = vm_new ();;
-let block = block_new Nil Nil Halt;;
-let program = program_new [block];;
+let program = program_new Nil Nil Halt;;
 let Vm (_, cells) = run vm program (S O);;
 
 match cells with
